theories/Presentation.v
@@ -1,0 +1,456 @@
+From Ltac2 Require Import Ltac2.
+From Ltac2 Require Import Std.
+
+From Ltac2 Require Fresh.
+From Ltac2 Require Import Control.
+From Ltac2 Require Import Message.
+From Ltac2 Require Import Std.
+From Ltac2 Require Import Printf.
+
+Import Ltac2.Notations.
+
+Require Import DlStalk.Lemmas.
+Require Import DlStalk.Tactics.
+Require Import DlStalk.LTS.
+Require Import DlStalk.Model.
+Require Import DlStalk.ModelData.
+Require Import DlStalk.Network.
+Require Import DlStalk.SRPC.
+Require Import DlStalk.Que.
+Require Import DlStalk.Locks.
+Require Import DlStalk.SRPC.
+Require Import DlStalk.SRPCNet.
+Require Import DlStalk.Transp.
+Require Import DlStalk.Sound.
+Require Import DlStalk.Compl.
+Require Import DlStalk.PresentationCompat.
+Require Import DlStalk.GenFramework.
+
+From Coq Require Import Strings.String.
+From Coq Require Import Lists.List.
+From Coq Require Import Structures.Equalities.
+Import ListNotations.
+Open Scope string_scope.
+
+Import Theory.
+Import SrpcDefs.
+
+(** * Introduction *)
+
+(** This module iterates through the major theorems, lemmas, definitions and
+notations that are used in or relevant to the paper. Some definitions have been
+edited in the paper for readability --- those which were simplified
+significantly have been proven to be equivalent to their counterparts used in
+this mechanisation.
+
+The project uses [Ltac2] as the proof language. [DlStalk.Tactics] contains
+definitions of custom tactics. *)
+
+(** Generic predicate for invariants over transitions. *)
+Print trans_invariant.
+(** Helper to mark unconditional invariants. *)
+Print always.
+
+(** * Modelling Networks of RPC Services *)
+
+(** ** Syntax of Processes, Queues, and Services *)
+
+(** Basic (see [DlStalk.ModelData]) *)
+Print Tag.
+Check Q : Tag.
+Check R : Tag.
+
+Check Val : Set.
+Check Name : Set.
+
+(** Process and service (see [DlStalk.Model]) *)
+Print Proc.
+Check Que Val.
+Print Serv.
+
+(** We abstract implementation of the network to a module type. Contrary to the
+paper, we do not use plain functions to represent networks, because that would
+require quite global extensionality which we do not need in general. (see
+[DlStalk.Network]) *)
+
+Print NET_MOD.
+
+(**  Creation of networks from functions *)
+Check NetMod.init : (Name -> Serv) -> NetMod.t Serv.
+
+(** Access *)
+Check NetMod.get : Name -> NetMod.t Serv -> Serv.
+(** Modification *)
+Check NetMod.put : Name -> Serv -> NetMod.t Serv -> NetMod.t Serv.
+
+(** Initialisation access axiom *)
+Check NetMod.init_get :
+        forall (f : Name -> Serv) (n : Name),
+          NetMod.get n (NetMod.init f) = f n.
+
+(** Fresh access axioms *)
+Check NetMod.get_put_eq :
+        forall n S N,
+          NetMod.get n (NetMod.put n S N) = S.
+Check NetMod.get_put_neq :
+        forall n n' S N,
+          n <> n' ->
+          NetMod.get n (NetMod.put n' S N) = NetMod.get n N.
+
+(** Update axioms *)
+Check NetMod.put_put_eq :
+        forall n S0 S1 N,
+          NetMod.put n S1 (NetMod.put n S0 N) = NetMod.put n S1 N.
+Check NetMod.put_put_neq :
+        forall n n' S0 S1 N,
+          n <> n' ->
+          NetMod.put n S1 (NetMod.put n' S0 N) = NetMod.put n' S0 (NetMod.put n S1 N).
+
+(** Overwrite axiom *)
+Check NetMod.put_get_eq :
+        forall n N, NetMod.put n (NetMod.get n N) N = N.
+
+(** Extensionality axiom *)
+Check NetMod.extensionality :
+        forall N0 N1,
+          (forall n, NetMod.get n N0 = NetMod.get n N1) -> N0 = N1.
+
+(** ** Semantics of Processes, Queues, Services, and Networks *)
+
+(** Generic definitions (see [DlStalk.LTS]) *)
+Print LTS.
+Print ptrans.
+Locate "_ =( _ )=> _".
+Locate "_ =[ _ ]=> _".
+
+(** Actions (see [DlStalk.Que] and [DlStalk.Model]) *)
+Print Act.
+Print QAct.
+
+(** Process, Queue and Service transitions. All are instances of the LTS class. *)
+Print ProcTrans.
+Print QTrans.
+Print STrans.
+
+Check trans_Serv : LTS PAct Serv.
+
+(** Network transitions. [NVTrans] is used as a helper to progress nodes within
+a network (see [DlStalk.Network]) *)
+Print NVTrans.
+Print NTrans.
+
+(** ** Locks and Deadlocks *)
+
+(** Paper-compatible definition of a service lock and deadset (see [DlStalk.Locks] and [DlStalk.NetLocks]) *)
+Print Paper.serv_lock.
+Print Paper.dead_set.
+
+(** Definitions used in the project *)
+Print proc_lock.
+Print serv_lock.
+Print lock_set.
+Print lock.
+Print dead_set.
+
+Check deadset_invariant : forall DS, trans_invariant (dead_set DS) always. (* TODO rename *)
+
+(** Compatibility of project and paper definitions (for SRPC services; see
+[DlStalk.SRPCNet]) *)
+Check serv_lock_eq : forall S n, (exists srpc, SRPC_serv srpc S) -> serv_lock [n] S <-> Paper.serv_lock n S.
+Check deadset_eq : forall (N : Net) (DS : Names), SRPC_net N -> dead_set DS N <-> Paper.dead_set DS N.
+
+(** Deadset-cycle equivalence (see [DlStalk.NetLocks]) *)
+Check deadset_dep_self : forall N : Net,
+          lock_uniq_type N -> lock_neq_nil_type N -> locks_dec_in N ->
+          forall DS, dead_set DS N -> exists n, In n DS /\ trans_lock N n n. (* TODO rename *)
+Check dep_self_deadset : forall N : Net,
+          lock_uniq_type N -> lock_neq_nil_type N ->
+          forall n, trans_lock N n n -> exists DS, In n DS /\ dead_set DS N.
+
+(** Well formed SRPC networks fulfill the prerequisites for deadset-cycle
+equivalence. (see [DlStalk.SRPCNet]) *)
+Import SrpcNet.
+Check SRPC_lock_set_uniq : forall [N : Net], SRPC_net N -> lock_uniq_type N.
+Check SRPC_lock_set_neq_nil : forall [N : Net], SRPC_net N -> lock_neq_nil_type N.
+Print locks_dec_in.
+Check well_formed_lock_dec  : forall (N : Net) n0 n1, well_formed N -> lock N n0 n1 \/ ~ lock N n0 n1.
+
+(** ** Single-Threaded RPC (SRPC) Services *)
+
+(** SRPC Working and SRPC Locked are stored separately from SRPC Ready (see [DlStalk.SRPC]) *)
+Print SRPC_State.
+Print SRPC_Busy_State.
+
+(** Paper-compatible definitions (see [DlStalk.PresentationCompat]) *)
+Print Paper.SRPCC.
+Print Paper.SRPCI.
+
+(**  Original SRPC property is defined slightly differently *)
+Check SRPC_eq.
+
+(** ** A Coq Framework for Modelling Erlang/OTP-Style SRPC Networks *)
+
+Section Framework.
+  (** The name "Thomas" does not refer to any of the authors. *)
+  Import Thomas.
+  Import Sound.
+  Import SrpcDefs.
+
+  (** Types for generic network configuration (see [DlStalk.GenFramework]) *)
+  Print ServiceConf.
+  Print InitConf.
+  Print NetConf.
+
+  (** The network is SRPC! *)
+  Check gen_net_SRPC : forall conf n, exists srpc, SRPC_serv srpc (NetMod.get n (gen_net conf)).
+
+  (** Example services and network *)
+  Print echo.
+  Print service.
+  Print example_net.
+
+  (** Can deadlock *)
+  Check can_deadlock : exists path N, (example_net =[ path ]=> N) /\ dead_set ["A"; "B"; "C"; "D"]%list N.
+End Framework.
+
+(** * Monitors, Instrumentation, and Transparency *)
+
+(** Probes. [MProbe] is an alias for a slightly more generic [MProbe'] (see [DlStalk.Compl]) *)
+Locate MProbe.
+Print MProbe'.
+Check origin : MProbe -> Name.
+Check lock_id : MProbe -> nat.
+
+(** Monitor messages (stored in the monitor queue) (see [DlStalk.Model]) *)
+Print EMsg.
+Locate MQue.
+
+(** Monitor state (see [DlStalk.Compl]) *)
+Locate MState.
+Print MState'.
+Check self : MState -> Name.
+Check locked : MState -> option Name.
+Check wait : MState -> list Name.
+Check lock_count : MState -> nat.
+Check alarm : MState -> bool.
+
+(** Monitor process (see [DlStalk.Model]) *)
+Print MProc.
+Check MRecv : MState -> MProc.
+Check MSend : (Name * Tag) -> MProbe -> MProc -> MProc.
+
+(** Monitored service (see [DlStalk.Model]) *)
+Print MServ.
+Check mserv_q.
+Check mserv_m.
+Check mserv_s.
+
+(** Transition of monitored services (see [DlStalk.Model]) *)
+Print MTrans.
+
+(** Instrumentation (see [DlStalk.Model]) *)
+Print mon_assg.
+Print instr.
+Check apply_instr.
+
+(** De-instrumentation (see [DlStalk.Model]) *)
+Print retract_recv.
+Print retract_send.
+Print serv_deinstr.
+Print deinstr.
+
+Check instr_inv : forall (i : instr) N, deinstr (i N) = N.
+
+(** Networks are generic, thus work for monitored services too (see [DlStalk.Network] and [DlStalk.Transp]) *)
+Check (NetMod.get : Name -> MNet -> MServ).
+Check (NetMod.get : Name -> Net  -> Serv).
+
+(** Transparency (see [DlStalk.Transp]) *)
+Check transp_sound : forall mnpath (MN0 MN1 : MNet),
+          MN0 =[ mnpath ]=> MN1 -> exists pnpath, deinstr MN0 =[ pnpath ]=> deinstr MN1.
+Check @transp_complete : forall path (i0 : instr) (N0 N1 : Net),
+          N0 =[ path ]=> N1 -> exists mpath (i1 : instr), i0 N0 =[ mpath ]=> i1 N1.
+
+
+(** * A Black-Box Distributed Deadlock Detection Algorithm *)
+
+Module Type Alg. (* We need to backdoor it a bit... *)
+  Declare Module Conf : DETECT_CONF.
+  Declare Module Params : MON_PARAMS(Conf).
+  Include Mh(Conf)(Params).
+
+  (** Implementation of the algorithm (see [DlStalk.Compl]) *)
+  Check mon_handle : EMsg -> MState -> MProc.
+  Print mon_handle.
+End Alg.
+
+(** * Correctness of Black-Box Distributed Deadlock Detection *)
+
+(** ** Monitor Correctness Criteria *)
+
+Section Correct.
+  Import Thomas.
+
+  (** Definition of correctness (see [DlStalk.GenFramework]) *)
+  Print detect_sound.
+  Print detect_complete.
+  Print detect_correct.
+End Correct.
+
+(** ** Finding and Proving Invariants *)
+
+(** *** Well-Formed SRPC Networks  *)
+
+(** Definition of the client relation and compatibility between the project and the paper (see [DlStalk.PresentationCompat]) *)
+Print Paper.client.
+Print serv_client.
+Check client_eq : forall n S, serv_client n S <-> Paper.client n S.
+
+(**  Well-formedness at the greatest detail (see [DlStalk.SRPCNet]) *)
+Print service_wf.
+
+Check service_wf_SRPC_inv : forall [srpc : SRPC_State] [S],
+    service_wf srpc S -> SRPC_serv srpc S.
+Check service_wf_Q_in_inv : forall [srpc : SRPC_State] [c v v' I I' P O],
+    service_wf srpc (serv I P O) ->
+    Deq (c, Q) v I I' ->
+    not (List.In (c, Q, v') I').
+Check service_wf_R_in_inv : forall [srpc : SRPC_State] [s s' v v' I I' P O],
+    service_wf srpc (serv I P O) ->
+    Deq (s, R) v I I' ->
+    not (List.In (s', R, v') I').
+Check service_wf_R_in_lock_inv : forall [srpc : SRPC_State] [s v I P O],
+    service_wf srpc (serv I P O) ->
+    In (s, R, v) I ->
+    exists c, srpc = Locked c s.
+Check service_wf_Q_out_lock_inv : forall [srpc : SRPC_State] [s v I P O],
+    service_wf srpc (serv I P O) ->
+    In (s, Q, v) O ->
+    exists c, srpc = Locked c s.
+Check service_wf_Q_out_last_inv : forall [srpc : SRPC_State] [s v I P O],
+    service_wf srpc (serv I P O) ->
+    ~ (In (s, Q, v) (List.removelast O)).
+Check service_wf_Q_out_uniq_inv : forall [srpc : SRPC_State] [c v v' I P O O'],
+    service_wf srpc (serv I P O) ->
+    Deq (c, R) v O O' ->
+    ~ (In (c, R, v') O').
+Check service_wf_R_Q_inv : forall [srpc : SRPC_State] [s v v' I P O],
+    service_wf srpc (serv I P O) ->
+    In (s, R, v) I -> not (In (s, Q, v') O).
+Check service_wf_Q_R_inv : forall [srpc : SRPC_State] [s v v' I P O],
+    service_wf srpc (serv I P O) ->
+    In (s, Q, v) O -> not (In (s, R, v') I).
+Check service_wf_lock_Q_inv : forall [c s I P O],
+    service_wf (Locked c s) (serv I P O) ->
+    O <> [] ->
+    exists v, In (s, Q, v) O.
+Check service_wf_Q_excl_R_inv : forall [srpc : SRPC_State] [c v v' I P O],
+    service_wf srpc (serv I P O) ->
+    In (c, Q, v) I ->
+    ~ In (c, R, v') O.
+Check service_wf_Q_excl_c_inv : forall [srpc : SRPC_State] [c v I P O],
+    service_wf srpc (serv I P O) ->
+    In (c, Q, v) I ->
+    ~ proc_client c P.
+Check service_wf_R_excl_Q_inv : forall [srpc : SRPC_State] [c v v' I P O],
+    service_wf srpc (serv I P O) ->
+    In (c, R, v) O ->
+    ~ In (c, Q, v') I.
+Check service_wf_R_excl_c_inv : forall [srpc : SRPC_State] [c v I P O],
+    service_wf srpc (serv I P O) ->
+    In (c, Q, v) I ->
+    ~ proc_client c P.
+Check service_wf_c_excl_Q_inv : forall [srpc : SRPC_State] [c v I P O],
+    service_wf srpc (serv I P O) ->
+    proc_client c P ->
+    ~ In (c, Q, v) I.
+Check service_wf_c_excl_R_inv : forall [srpc : SRPC_State] [c v I P O],
+    service_wf srpc (serv I P O) ->
+    proc_client c P ->
+    ~ In (c, R, v) O.
+
+Print well_formed.
+Check trans_invariant_well_formed : trans_invariant well_formed always. (* TODO rename *)
+
+(** *** Monitor Knowledge Invariant for Sound Deadlock Detection  *)
+
+(** (see [DlStalk.Sound]) *)
+Print sends_to.
+Print sends_to_mon.
+Check stm_find : forall n p M, sends_to_mon (MSend (n, R) p M) n p.
+Check stm_seek : forall n nc' p p' M,
+    nc' <> (n, R) \/ p <> p' ->
+    sends_to_mon M n p ->
+    sends_to_mon (MSend nc' p' M) n p.
+
+Print KIS.
+
+Check KIS_well_formed : forall [MN], KIS MN -> well_formed '' MN.
+Check KIS_self : forall [MN], KIS MN -> forall n0, self (MN n0) = n0.
+Check KIS_locked : forall [MN], KIS MN -> forall n0 n1, locked (MN n0) = Some n1 -> lock '' MN n0 n1 \/ exists v, List.In (MqRecv (n1, R) v) (mserv_q (MN n0)).
+Check KIS_wait : forall [MN], KIS MN -> forall n0 n1, List.In n0 (wait (MN n1)) -> lock '' MN n0 n1.
+Check KIS_sendp : forall [MN], KIS MN -> forall n0 n1 p, sends_to MN n1 n0 p -> lock '' MN n0 n1.
+Check KIS_lock_id_sendp : forall [MN], KIS MN -> forall n0 n1 p, sends_to MN n0 n1 p -> (lock_id p <= lock_count (MN (origin p)))%nat.
+Check KIS_lock_id_recvp : forall [MN], KIS MN -> forall n0 n1 p, List.In (MqProbe (n1, R) p) (mserv_q (MN n0)) -> (lock_id p <= lock_count (MN (origin p)))%nat.
+Check KIS_sendp_active : forall [MN], KIS MN -> forall n0 n1 n2, sends_to MN n1 n0 (active_probe_of MN n2) -> locked (MN n2) <> None -> trans_lock '' MN n0 n2.
+Check KIS_recvp_active : forall [MN], KIS MN -> forall n0 n1 n2, List.In (active_ev_of MN n2 n0) (mserv_q (MN n1)) -> locked (MN n0) <> None -> trans_lock '' MN n1 n0.
+Check KIS_alarm : forall [MN], KIS MN -> forall n, alarm (MN n) = true -> trans_lock '' MN n n.
+
+Check KIS_invariant : trans_invariant KIS always.
+Check detection_soundness : forall (i0 : instr) N0 MN1 mpath n,
+    KIS (i0 N0) -> (i0 N0 =[ mpath ]=> MN1) -> alarm (MN1 n) = true ->
+    exists DS, dead_set DS '' MN1 /\ In n DS. (* TODO rename *)
+
+(** Monitor message (in monitor queue) holding an active probe *)
+Print active_ev_of.
+
+(** *** Monitor Knowledge Invariant for Complete Deadlock Detection  *)
+
+(**  (see [DlStalk.Compl]) *)
+
+Print sends_probe.
+Print ac. (* TODO rename *)
+Print KIC.
+
+Check KIC_invariant : trans_invariant KIC always.
+Check ac_to_alarm : forall MN0 n,
+    KIC MN0 ->
+    ac n MN0 ->
+    trans_lock '' MN0 n n ->
+    exists DS mpath MN1,
+      (MN0 =[ mpath ]=> MN1) /\ dead_set DS '' MN0 /\ detect_path DS mpath /\ alarm (MN1 n) = true.
+
+Check detection_complete : forall (i0 : instr) N0 MN1 mpath0 DS,
+    KIC (i0 N0) ->
+    (i0 N0 =[ mpath0 ]=> MN1) ->
+    dead_set DS '' MN1 ->
+    exists mpath1 MN2 n,
+      (MN1 =[ mpath1 ]=> MN2) /\ In n DS /\ alarm (MN2 n) = true.
+
+(** ** Correct Monitoring for Erlang << gen_server >> -Style Applications  *)
+
+Section Correct.
+  Import Thomas. Import Sound.
+
+  (** The framework is correct (see [DlStalk.GenFramework]) *)
+  Print gen_instr.
+
+  Check gen_net_well_formed : forall conf, well_formed (gen_net conf).
+  Check gen_KIS : forall conf : NetConf, KIS (gen_instr (gen_net conf)).
+  Check gen_KIC : forall conf : NetConf, KIC (gen_instr (gen_net conf)).
+
+  Check gen_correct : forall conf, detect_correct (gen_net conf) gen_instr.
+
+  (** Let's say it again *)
+  Check gen_correct : forall conf,
+      let N0 := gen_net conf in
+      and
+        (forall path' MN1 n,
+            (gen_instr N0 =[ path' ]=> MN1) /\ alarm (MN1 n) = true ->
+            exists DS, In n DS /\ dead_set DS '' MN1
+        )
+        (forall path0' MN1 DS,
+            (gen_instr N0 =[ path0' ]=> MN1) -> dead_set DS '' MN1 ->
+            exists path1' MN2 n, (MN1 =[ path1' ]=> MN2) /\ In n DS /\ alarm (MN2 n) = true
+        ).
+End Correct.
